more in ListT

dialectica/ListT.v
@@ -1,4 +1,4 @@
-Require Extensionality.
+Require Import Extensionality.
 
 (** Implementation of the List monad transformer in Coq. *)
 
@@ -7,16 +7,32 @@ Set Implicit Arguments.
 (** We use Mersenne induction to ensure that even if T may not be positive, that
     does not impede the writing of such a type. *)
 
-Inductive listT R (T : Type -> Type) A :=
-| NodeT : forall S, (S -> R + nodeT R T A) -> T S -> listT R T A
+Inductive PlistT R (T : Type -> Type) A :=
+| NodeT : forall S, (S -> R + PnodeT R T A) -> T S -> PlistT R T A
 
-with nodeT R (T : Type -> Type) A :=
-| Nil : nodeT R T A
-| Cons : A -> listT R T A -> nodeT R T A.
+with PnodeT R (T : Type -> Type) A :=
+| Nil : PnodeT R T A
+| Cons : A -> PlistT R T A -> PnodeT R T A.
+
+Definition listT T A := PlistT False T A.
+Definition nodeT T A := PnodeT False T A.
 
 Arguments Nil [_ _ _].
 
-Fixpoint map {R T A B} (f : A -> B) (l : listT R T A) : listT R T B
+Fixpoint map {T A B} (f : A -> B) (l : listT T A) : listT T B
+with map_node {T A B} (f : A -> B) (n : nodeT T A) : nodeT T B.
+Proof.
++ destruct l as [S k n]; exists S.
+  - intros s; destruct (k s) as [[]|N].
+    right; apply (map_node _ A B f N).
+  - exact n.
++ destruct n as [|x l].
+  - apply Nil.
+  - apply Cons; [exact (f x)|].
+    apply (map _ _ _ f l).
+Defined.
+
+(* Fixpoint map {R T A B} (f : A -> B) (l : listT R T A) : listT R T B
 with map_node {R T A B} (f : A -> B) (n : nodeT R T A) : nodeT R T B.
 Proof.
 + destruct l as [S k n]; exists S.
@@ -28,16 +44,30 @@ Proof.
   - apply Nil.
   - apply Cons; [exact (f x)|].
     apply (map _ _ _ _ f l).
-Defined.
+Defined.*)
 
 Section Ops.
 
-Context (R : Type) (T : Type -> Type).
+Context (T : Type -> Type).
 Variable lift : forall {A}, A -> T A.
 Variable bind : forall {A B}, (A -> T B) -> (T A -> T B).
 
-Fixpoint fold_right {A B} (f : B -> A -> A) (accu : T A) (l : listT R T B) : T (R + A)
-with fold_right_node {A B} (f : B -> A -> A) (accu : T A) (n : nodeT R T B) : T (R + A).
+Fixpoint fold_right {A B} (f : B -> A -> T A) (accu : T A) (l : listT T B) : T A
+with fold_right_node {A B} (f : B -> A -> T A) (accu : T A) (n : nodeT T B) : T A.
+Proof.
++ destruct l as [S k s].
+  apply (@bind S); [clear s|exact s].
+  intros s; destruct (k s) as [[]|n].
+  apply (fold_right_node _ _ f accu n).
++ destruct n as [|x l].
+  - exact accu.
+  - pose (ans := fold_right _ _ f accu l).
+    refine (bind _ ans); clear ans accu; intros accu.
+    apply (f x accu).
+Defined.
+
+(* Fixpoint fold_right {A B} (f : B -> A -> T A) (accu : T A) (l : listT R T B) : T (R + A)
+with fold_right_node {A B} (f : B -> A -> T A) (accu : T A) (n : nodeT R T B) : T (R + A).
 Proof.
 + destruct l as [S k s].
   apply (@bind S); [clear s|exact s].
@@ -49,7 +79,22 @@ Proof.
   - pose (ans := fold_right _ _ f accu l).
     refine (bind _ ans); clear ans accu; intros [r|accu].
     { apply lift, inl, r. }
-    { apply lift, inr, (f x accu). }
-Defined.
+    { refine (bind _ (f x accu)); intros ans; apply lift, inr, ans. }
+Defined.*)
 
+(* Definition collapse {A} (m : T (listT T A)) : listT T A.
+Proof.
+exists (nodeT T A); [exact inr|].
+refine (bind _ m).
+intros [S k s].
+refine (bind _ s); clear s; intros s.
+destruct (k s) as [[]|n]; apply lift, n.
+Defined.*)
+
+Definition nil {A} : (listT T A) := NodeT (fun _ => inr Nil) (lift tt).
+Definition cons {A} (x : A) (l : listT T A) := NodeT (fun _ => inr (Cons x l)) (lift tt).
+
+(* Lemma toto : forall A B (f : A -> B) l,
+  map f l ≅ fold_right (fun x accu => lift (cons (f x) accu)) (lift nil) l.
+ *)
 End Ops.
